Proofs.v
@@ -14,6 +14,11 @@ Hint Extern 10 => varsdec : set.
 
 Arguments Vars.union !_ !_.
 
+Lemma vars_mem_false x vs : ~Vars.In x vs -> Vars.mem x vs = false.
+Proof.
+ rewrite <- Vars.mem_spec. now case Vars.mem.
+Qed.
+
 Lemma InA_In {A} x (l:list A) : InA eq x l <-> In x l.
 Proof.
  split.
